src/Rdf.v
@@ -570,7 +570,7 @@ Section Rdf.
             {in ts &, injective (relabeling_triple mu)}.
         Proof.
           move=> mu_inj; case=> sx ps ox ? ?; case=> sy py oy ? ? /= /mem_triple_terms_ts /= /and3P[memsx mempx memox] /mem_triple_terms_ts /= /and3P[memsy mempy memoy] [] eqs eqp eqo.
-            by apply triple_inj=> /=; apply (relabeling_term_inj_terms_ts mu_inj)=> //.
+          by apply triple_inj=> /=; apply (relabeling_term_inj_terms_ts mu_inj)=> //.
         Qed.
 
         Lemma can_bts_can_rtbs ts (mu nu: B -> B) :
@@ -783,7 +783,10 @@ Section Rdf.
         Lemma is_pre_iso_ts_inv ts1 ts2 mu :
           is_pre_iso_ts ts1 ts2 mu ->
             exists nu, is_pre_iso_ts ts2 ts1 nu /\
-                    map (nu \o mu) (get_bts ts1) = get_bts ts1.
+                    map (nu \o mu) (get_bts ts1) = get_bts ts1
+                                                           .
+                       (* /\ *)
+                       (*   map (mu \o nu) (get_bts ts2) = get_bts ts2. *)
         Proof.
         wlog dflt :/ B.
           move=> hwlog; rewrite /is_pre_iso_ts/get_b/bnode_map_bij.
@@ -797,16 +800,25 @@ Section Rdf.
           have {rhoP} rhoP : [seq (rho \o mu) i | i <- get_bts ts1] = get_bts ts2.
           rewrite -map_comp in rhoP; apply: rhoP; first by rewrite (perm_uniq mu_pre_iso).
             by rewrite (perm_size mu_pre_iso).
-          have {hwlog} [tau [/and3P[_ _ tauP1] tauP2]] := hwlog _ rhoP.
+          have [tau [/and3P[_ _ tauP1] tauP2]] := hwlog _ rhoP.
+          (* have [tau [/and3P[_ _ tauP1] [tauP21 tauP22]]] := hwlog _ rhoP. *)
           exists (tau \o rho); split=> //.
           rewrite /bnode_map_bij perm_sym !uniq_get_bts -tauP2 /=.
+          (* rewrite /bnode_map_bij perm_sym !uniq_get_bts -tauP21 /=. *)
           have:=  (perm_map (tau \o rho) mu_pre_iso).
           by rewrite -map_comp.
+          (* split. *)
+          (* by rewrite -compA tauP21. *)
+          (* rewrite -rhoP -map_comp. rewrite /=. *)
         have [nu nuP] := map_of_seq (get_bts ts2) (get_bts ts1) dflt.
         have  {nuP} nuP : [seq nu i | i <- get_bts ts2] = get_bts ts1.
           by apply: nuP=> //; rewrite -map_mu size_map.
         exists nu; split=> //.
         - rewrite /bnode_map_bij !uniq_get_bts nuP; exact: perm_refl.
+        (* have invP : *)
+        (*   [seq (mu \o nu) i | i <- get_bts ts2] = get_bts ts2. *)
+        (*   apply (f_equal (map mu)) in nuP. *)
+        (*   by rewrite (map_comp mu nu) nuP. *)
         by rewrite map_comp map_mu.
         Qed.
 
@@ -881,23 +893,37 @@ Section Rdf.
       Definition is_iso_ts ts1 ts2 mu :=
         [&& is_pre_iso_ts ts1 ts2 mu,
           uniq (relabeling_seq_triple mu ts1) &
-            perm_eq (relabeling_seq_triple mu ts1) ts2].
+            perm_eq (relabeling_seq_triple mu ts1) ts2] /\
+          (forall t, forall wf_s wf_p, @mkTriple I B L (relabeling_term mu (subject t)) (predicate t) (relabeling_term mu (object t)) wf_s wf_p \in ts2 -> t \in ts1).
 
-      Definition is_iso g1 g2 mu :=
+
+      Definition is_iso g1 g2 mu : Prop :=
         [&& is_pre_iso g1 g2 mu,
           uniq (relabeling_seq_triple mu g1) &
-            perm_eq (relabeling_seq_triple mu g1) g2].
+            perm_eq (relabeling_seq_triple mu g1) g2] /\
+          (forall t, forall wf_s wf_p, @mkTriple I B L (relabeling_term mu (subject t)) (predicate t) (relabeling_term mu (object t)) wf_s wf_p \in g2 -> t \in g1).
+
 
       Definition iso_ts ts1 ts2 := exists mu, @is_iso_ts ts1 ts2 mu.
       Definition iso g1 g2 := iso_ts g1 g2.
 
       Remark is_iso_is_pre_iso g1 g2 mu: is_iso g1 g2 mu -> is_pre_iso g1 g2 mu.
-      Proof. by case/and3P. Qed.
+      Proof. by move=> [/and3P[piso]]. Qed.
 
       Definition iso_refl g : iso g g.
-      Proof. exists id; rewrite /is_iso/is_iso_ts/is_pre_iso_ts/bnode_map_bij.
-             case g=> g' ug /=.
-             by rewrite uniq_get_bts! relabeling_seq_triple_id ug  /= /is_pre_iso/is_pre_iso_ts map_id !perm_refl.
+      Proof. exists id; split.
+             + rewrite /is_iso/is_iso_ts/is_pre_iso_ts/bnode_map_bij.
+               case g=> g' ug /=.
+               by rewrite uniq_get_bts! relabeling_seq_triple_id ug  /= /is_pre_iso/is_pre_iso_ts map_id !perm_refl.
+             + move=> t wfs wfp.
+               suffices -> : {|
+                               subject := relabeling_term id (subject t);
+                               predicate := predicate t;
+                               object := relabeling_term id (object t);
+                               subject_in_IB := wfs;
+                               predicate_in_I := wfp
+                             |} = t. done.
+               by apply triple_inj; rewrite //= relabeling_term_id.
       Qed.
 
       Section eqb_rdf_perm_eq.
@@ -947,51 +973,325 @@ Section Rdf.
         exists id.
         have usid: uniq (relabeling_seq_triple id ts1) by rewrite relabeling_seq_triple_id.
         rewrite /is_iso/is_iso_ts usid /is_pre_iso/is_pre_iso_ts/bnode_map_bij.
-        rewrite map_id relabeling_seq_triple_id /= !uniq_get_bts ; apply/andP; split=> //.
-        - exact: peq_get_bts.
+        rewrite map_id relabeling_seq_triple_id /= !uniq_get_bts /=; split.
+        + apply/andP; split=> //=; exact: peq_get_bts.
+        + move=> t wfs wfp.
+          suffices -> : {|
+                          subject := relabeling_term id (subject t);
+                          predicate := predicate t;
+                          object := relabeling_term id (object t);
+                          subject_in_IB := wfs;
+                          predicate_in_I := wfp
+                        |} = t. by rewrite (perm_mem H).
+          by apply triple_inj; rewrite //= relabeling_term_id.
       Qed.
 
 
       Remark eqiso g1 g2 : eqb_rdf g1 g2 -> iso g1 g2.
       Proof. by apply : eqiso_ts (uniq_rdf_graph _). Qed.
 
+      Lemma projs_rel (t : triple I B L) (B2 : Type) (mu : B -> B2) :  (subject (relabeling_triple mu t)) = relabeling_term mu (subject t).
+      Proof. by case:t. Qed. 
+
+      Lemma projp_rel (t : triple I B L) (B2 : Type) (mu : B -> B2) :  (predicate (relabeling_triple mu t)) = relabeling_term mu (predicate t).
+      Proof. by case:t. Qed. 
+
+      Lemma projo_rel (t : triple I B L) (B2 : Type) (mu : B -> B2) :  (object (relabeling_triple mu t)) = relabeling_term mu (object t).
+        Proof. by case:t. Qed. 
+
+
+      Lemma pred_relab (t : triple I B L) (mu : B -> B) :
+        predicate (relabeling_triple mu t) = predicate t.
+      Proof. by case: t=> ? [] ? //. Qed.
+
+      (* Lemma contraPNN : forall [P : Prop] [b : bool], (~ P -> b) -> ~~ b -> P. *)
+      (* Proof. move=> P b //. apply contraPN in b. *)
+
+      Lemma not_perm_eq (T : eqType) (s1 s2: seq T) :
+        uniq s1 -> uniq s2 -> size s1 = size s2 -> negb (perm_eq s1 s2) -> exists (t : T), (t \in s1) && (t \notin s2).
+      Proof. move=> us1 us2 eqsize.
+      Admitted.
+
       Lemma iso_ts_sym ts1 ts2 (u1 : uniq ts1) (u2 : uniq ts2) : iso_ts ts1 ts2 <-> iso_ts ts2 ts1.
       Proof.
-        suffices imp h1 h2 : uniq h1 -> iso_ts h1 h2 -> iso_ts h2 h1 by split; exact: imp.
-        move=> uh1; case=> mu /and3P[pre_iso_mu uniq_relab perm_relab].
-        move:(is_pre_iso_ts_inv pre_iso_mu); rewrite /pre_iso/is_pre_iso; move=> [nu [pre_iso_nu /map_comp_in_id_ts/can_bs_can_rtbs nuP]].
-        exists nu.
-        rewrite /is_iso/is_iso_ts pre_iso_nu.
-        suffices peq : perm_eq (relabeling_seq_triple nu h2) h1.
-          by move/(perm_eq_relab_uniq_ts uh1) : peq => [-> ->].
-        move: perm_relab; rewrite perm_sym=> /(perm_map (relabeling_triple nu))=> perm_relab.
-        by apply: perm_trans perm_relab _; rewrite relabeling_triple_map_comp map_id_in //.
+        suffices imp G H : uniq G -> iso_ts G H -> iso_ts H G by split; exact: imp.
+        move=> /= uG; case=> mu [/and3P[pre_iso_mu uniq_relab perm_relab] mem_eq].
+        move:(is_pre_iso_ts_inv pre_iso_mu); rewrite /pre_iso/is_pre_iso; move=> [nu [pre_iso_nu eq]].
+        have eq2 := eq.
+        move: eq=> /map_comp_in_id_ts mu_inv.
+        have /can_bs_can_rtbs eq := mu_inv.
+          rewrite /iso_ts/is_iso/is_iso_ts.
+          suffices [rho [/andP[piso_rho peq_rho] mu_part]]: exists rho : B -> B,
+              (is_pre_iso_ts H G rho && perm_eq (relabeling_seq_triple rho H) G) /\
+                forall b, rho b \in (get_bts G) -> b \in get_bts H.
+        (* + set nu2 := (fun b => if (b \in (get_bts h2)) then nu b else b). *)
+          (* suffices H4 : forall b, nu2 b \in (get_bts h1) -> b \in get_bts h2. *)
+          (* exists nu2. *)
+          (* rewrite /is_iso/is_iso_ts. *)
+          (* suffices /andP[piso_nu2 peq] : *)
+          (*   (is_pre_iso_ts h2 h1 nu2) && perm_eq (relabeling_seq_triple nu2 h2) h1. *)
+            exists rho; split.
+            + by move/(perm_eq_relab_uniq_ts uG) : peq_rho => [-> ->]; rewrite piso_rho.
+            + move=> t wfs wfp.
+              suffices -> : {|
+                              subject := relabeling_term rho (subject t);
+                              predicate := predicate t;
+                                                   object := relabeling_term rho (object t);
+                                                             subject_in_IB := wfs;
+                                                                              predicate_in_I := wfp
+                         |} = relabeling_triple rho t.
+                (* suffices power : forall b, nu2 b \in (get_bts h1) -> b \in (get_bts h2). *)
+                  suffices /(_ I L) SH : forall s s', s' \in get_bts H -> Bnode (rho s) = Bnode (rho s') -> s \in get_bts H.
+                    rewrite -(perm_mem peq_rho)=> /mapP/=[t' t'inh2 eqtt' ].
+                    have /and3P[/eqP eqs /eqP eqp /eqP eqo] := triple_case eqtt'.
+                    rewrite !projo_rel in eqo.
+                    rewrite !projs_rel in eqs.
+                    rewrite !projp_rel in eqp.
+                    case_eq ((is_bnode (subject t)) || (is_bnode (object t))).
+                    + move=> /orP[].
+                  case: t t' t'inh2 wfs wfp eqtt' eqo eqs eqp=> //= [[]]s p o sib pii; case=> //= [[]]s' p' o' sib' pii' //= t'inh2 wfs wfp eqtt' eqo eqs eqp.
+                  suffices s'inh2 : s' \in (get_bts H).
+                    have sinh2 := SH s s' s'inh2 eqs.
+                    apply is_pre_iso_ts_inj2 in piso_rho.
+                    move: eqs=> []/(piso_rho _ _ sinh2 s'inh2) eqs.
+                      suffices -> : {| subject := Bnode s; predicate := p; object := o; subject_in_IB := sib; predicate_in_I := pii |} = {| subject := Bnode s'; predicate := p'; object := o'; subject_in_IB := sib'; predicate_in_I := pii' |}.
+                        by [].
+                      apply triple_inj=> //; rewrite eqs //=.
+                      + by move: p p' pii pii' eqp t'inh2 eqtt' wfp=> []p []p'.
+                      + move: o o' eqo t'inh2 eqtt' wfp=> []o []o' //= eqo t'inh2.
+                        suffices o'inh2 : o' \in (get_bts H).
+                          have oinh2 := SH o o' o'inh2 eqo.
+                          by move: eqo=> []/(piso_rho _ _ oinh2 o'inh2) eqo _ _; rewrite eqo.
+                        suffices bnode_in :  Bnode o' \in bnodes_triple  {|
+                                                         subject := Bnode s';
+                                                           predicate := p';
+                                                           object := Bnode o';
+                                                           subject_in_IB := sib';
+                                                           predicate_in_I := pii'
+                                                         |}.
+                          by apply (mem_ts_mem_triple_bts t'inh2 bnode_in).
+                        by rewrite /bnodes_triple/terms_triple filter_undup mem_undup -mem_rev -filter_rev /= in_cons eqxx.
+                      suffices bnode_in :  Bnode s' \in bnodes_triple  {|
+                                                       subject := Bnode s';
+                                                         predicate := p';
+                                                         object := o';
+                                                         subject_in_IB := sib';
+                                                         predicate_in_I := pii'
+                                                       |}.
+                        by apply (mem_ts_mem_triple_bts t'inh2 bnode_in).
+                      by rewrite /bnodes_triple/terms_triple filter_undup mem_undup /= in_cons eqxx.
+                      (* === *)
+                  case: t t' t'inh2 wfs wfp eqtt' eqo eqs eqp=> //= s p []o sib pii; case=> //= s' p' []o' sib' pii' //= t'inh2 wfs wfp eqtt' eqo eqs eqp.
+                  suffices o'inh2 : o' \in (get_bts H).
+                    have oinh2 := SH o o' o'inh2 eqo.
+                    apply is_pre_iso_ts_inj2 in piso_rho.
+                    move: eqo=> []/(piso_rho _ _ oinh2 o'inh2) eqo.
+                      suffices -> : {| subject := s; predicate := p; object := Bnode o; subject_in_IB := sib; predicate_in_I := pii |} = {| subject := s'; predicate := p'; object := Bnode o'; subject_in_IB := sib'; predicate_in_I := pii' |}.
+                        by [].
+                      apply triple_inj=> //; rewrite eqo //=; first last.
+                      + by move: p p' pii pii' eqp t'inh2 eqtt' wfp=> []p []p'.
+                      + move: s s' eqs sib sib' eqtt' wfs t'inh2=> []s []s' //= eqs sib sib' eqtt' wfs t'inh2.
+                        suffices s'inh2 : s' \in (get_bts H).
+                          have sinh2 := SH s s' s'inh2 eqs.
+                          by move: eqs=> []/(piso_rho _ _ sinh2 s'inh2) ->.
+                        suffices bnode_in :  Bnode s' \in bnodes_triple  {|
+                                                         subject := Bnode s';
+                                                           predicate := p';
+                                                           object := Bnode o';
+                                                           subject_in_IB := sib';
+                                                           predicate_in_I := pii'
+                                                         |}.
+                          by apply (mem_ts_mem_triple_bts t'inh2 bnode_in).
+                        by rewrite /bnodes_triple/terms_triple filter_undup mem_undup in_cons eqxx.
+                      suffices bnode_in :  Bnode o' \in bnodes_triple
+                                                         {|
+                                                                   subject := s';
+                                                                   predicate := p';
+                                                                   object := Bnode o';
+                                                                   subject_in_IB := sib';
+                                                                   predicate_in_I := pii'
+                                                                 |}.
+                        by apply (mem_ts_mem_triple_bts t'inh2 bnode_in).
+                      by rewrite /bnodes_triple/terms_triple filter_undup mem_undup -mem_rev -filter_rev /= in_cons eqxx.
+                    rewrite Bool.orb_false_iff.
+                    case: t t' t'inh2 wfs wfp eqtt' eqo eqs eqp=> //= [[]]s []p []o sib pii; case=> //= [[]]s' []p' []o' sib' pii' //= t'inh2 wfs wfp eqtt' eqo eqs eqp [] // _ _.
+                    suffices -> : {|
+    subject := Iri s;
+    predicate := Iri p;
+    object := Iri o;
+    subject_in_IB := sib;
+    predicate_in_I := pii
+                               |} = {|
+                                      subject := Iri s';
+                                      predicate := Iri p';
+                                      object := Iri o';
+                                      subject_in_IB := sib';
+                                      predicate_in_I := pii'
+                                    |}.
+                    by [].
+                    by apply triple_inj.
+                    suffices -> : {|
+    subject := Iri s;
+    predicate := Iri p;
+    object := Lit o;
+    subject_in_IB := sib;
+    predicate_in_I := pii
+                               |} = {|
+                                      subject := Iri s';
+                                      predicate := Iri p';
+                                      object := Lit o';
+                                      subject_in_IB := sib';
+                                      predicate_in_I := pii'
+                                    |}.
+                    by [].
+                    by apply triple_inj.
+                  + move=> ? ? b b' /(map_f (rho)).
+                    move: piso_rho=> /and3P[_ _ /perm_mem ->] rho_b'in []eq_rho.
+                    by move: rho_b'in; rewrite -eq_rho=> /mu_part.
+                + apply triple_inj=> //=.
+                  - by rewrite projs_rel.
+                  - by rewrite projp_rel; case: (predicate t) wfp.
+                  - by rewrite projo_rel.
+              + rewrite /is_pre_iso_ts/bnode_map_bij in pre_iso_mu.
+                move: pre_iso_mu => /and3P[_ _ pre_iso_mu].
+                suffices [rho [piso_rho [rho_part eq1_rho_nu]]]: exists rho, is_pre_iso_ts H G rho /\
+                                          (forall b : B, rho b \in get_bts G -> b \in get_bts H) /\
+                                         {in (get_bts H), nu =1 rho}.
+                 exists rho. rewrite piso_rho; split=> //=.
+            move: perm_relab; rewrite perm_sym=> /(perm_map (relabeling_triple rho))=> perm_relab.
+            apply: perm_trans perm_relab _; rewrite relabeling_triple_map_comp map_id_in //.
+            suffices : {in (get_bts G), (rho \o mu) =1 (nu \o mu)}.
+              + move=> eq1_rhomu_numu /= t tin; apply triple_inj.
+                + rewrite projs_rel; move: t tin; case=> [[]]s p o sib pii //=.
+                  suffices bin : Bnode s \in bnodes_triple  {| subject := Bnode s; predicate := p; object := o; subject_in_IB := sib; predicate_in_I := pii |}.
+                    move=> /mem_ts_mem_triple_bts /(_ bin) sin.
+                    congr Bnode. rewrite /comp in eq1_rhomu_numu mu_inv.
+                    by rewrite eq1_rhomu_numu // mu_inv.
+                  by rewrite /bnodes_triple/terms_triple filter_undup mem_undup in_cons eqxx.
+                + by rewrite projp_rel; move: t tin; case=> [[]]s []p o sib pii.
+                + rewrite projo_rel; move: t tin; case=> s p []o sib pii //=.
+                  suffices bin : Bnode o \in bnodes_triple {| subject := s; predicate := p; object := Bnode o; subject_in_IB := sib; predicate_in_I := pii |}.
+                    move=> /mem_ts_mem_triple_bts /(_ bin) sin.
+                    congr Bnode. rewrite /comp in eq1_rhomu_numu mu_inv.
+                    by rewrite eq1_rhomu_numu // mu_inv.
+                  by rewrite /bnodes_triple/terms_triple filter_undup mem_undup -mem_rev -filter_rev in_cons eqxx.
+                move=> b bin.
+                suffices mub_inH : mu b \in get_bts H.
+                  by rewrite /= -eq1_rho_nu // mu_inv.
+                by apply (map_f mu) in bin; rewrite (perm_mem pre_iso_mu) in bin.
+                case_eq (perm_eq (get_bts H) (get_bts G)).
+                set rho := (fun b => if (b \in (get_bts H)) then nu b else b).
+                suffices eq1_nu_rho : {in (get_bts H), nu =1 rho}.
+                exists rho; split.
+                  + apply /and3P; rewrite !uniq_get_bts /=; apply /and3P=> /=.
+                    apply eq_in_map in eq1_nu_rho; rewrite -eq1_nu_rho.
+                    by move: pre_iso_nu=> /and3P[_ _ ->].
+                  + split=> //.
+                    rewrite /rho=> b.
+                    case_eq (b \in get_bts H)=> //.
+                    by rewrite (perm_mem H0)=> ->.
+                  + by rewrite /rho => b ->.
+                move=> not_peq.
+                suffices  [b0 /andP[bin_H bnin_G]] : exists b, (b \in (get_bts H)) && (negb (b \in (get_bts G))).
+                set rho := (fun b => if (b \in (get_bts H)) then nu b else b0).
+                suffices eq1_nu_rho : {in (get_bts H), nu =1 rho}.
+                  exists rho; split=> //.
+                  + apply /and3P; rewrite !uniq_get_bts /=; apply /and3P=> /=.
+                    apply eq_in_map in eq1_nu_rho; rewrite -eq1_nu_rho.
+                    by move: pre_iso_nu=> /and3P[_ _ ->].
+                  + split=> //.
+                    rewrite /rho=> b.
+                    case_eq (b \in get_bts H)=> //.
+                    by move=> _; apply contraTT.
+                    rewrite /rho=> b.
+                    case_eq (b \in get_bts H)=> //.
+                    eapply (@not_perm_eq _ (get_bts H) (get_bts G))=> //.
+                    move: pre_iso_mu=> [/perm_size pre_iso_mu].
+                    by rewrite size_map in pre_iso_mu.
+                    by rewrite not_peq.
       Qed.
 
       Lemma iso_sym g1 g2 : iso g1 g2 <-> iso g2 g1.
       Proof. by apply: iso_ts_sym (uniq_rdf_graph _) (uniq_rdf_graph _). Qed.
 
+      Lemma eq_mem_in (T : eqType) (s : seq T) (a b : T) : a = b -> a \in s -> b \in s.
+      Proof. by move => ->. Qed.
+
       Lemma iso_ts_trans ts1 ts2 ts3 : iso_ts ts1 ts2 -> iso_ts ts2 ts3 -> iso_ts ts1 ts3.
-      Proof. rewrite /iso/is_iso; move=> [mu12 /and3P[pre_iso12 urel12 perm12]] [mu23 /and3P[pre_iso23 urel23 perm23]].
+      Proof. rewrite /iso/is_iso; move=> [mu12 [/and3P[pre_iso12 urel12 perm12] mu12_part]] [mu23 [/and3P[pre_iso23 urel23 perm23] mu23_part]].
              exists (mu23 \o mu12).
              suffices ucomp: uniq (relabeling_seq_triple (mu23 \o mu12) ts1).
-             apply /and3P; split=> //.
-             + by apply: is_pre_iso_ts_trans pre_iso12 pre_iso23.
-             + by apply : perm_eq_comp perm12 perm23.
-             + rewrite -relabeling_seq_triple_comp /relabeling_seq_triple.
-               have /eq_uniq -> //: size [seq relabeling_triple mu23 i | i <- [seq relabeling_triple mu12 i | i <- ts1]] =
-                             size (relabeling_seq_triple mu23 ts2).
-               by move: perm12=> /perm_size; rewrite !size_map.
-               by apply eq_mem_map; apply perm_mem.
+             split.
+               apply /and3P; split=> //.
+               + by apply: is_pre_iso_ts_trans pre_iso12 pre_iso23.
+               + by apply : perm_eq_comp perm12 perm23.
+               + move=> t wfs wfp tin.
+                 (* suffices -> : {| *)
+                 (*                 subject := relabeling_term (mu23 \o mu12) (subject t); *)
+                 (*                 predicate := predicate t; *)
+                 (*                 object := relabeling_term (mu23 \o mu12) (object t); *)
+                 (*                 subject_in_IB := wfs; *)
+                 (*                 predicate_in_I := wfp *)
+                 (*               |} = relabeling_triple mu23 (relabeling_triple mu12 t). *)
+
+                 move: mu23_part=> /(_ (relabeling_triple mu12 t)).
+                 have wfs2 := wfs.
+                 rewrite -projs_rel relabeling_triple_comp projs_rel in wfs2.
+                 move=> /(_ wfs2).
+                 have wfp2 := wfp.
+                 have /(_ I L t) /iffLR /(_ wfp2) wfp3 := (relabeling_triple_preserves_is_in_i mu12).
+                 move=> /(_ wfp3).
+                 suffices -> : {|
+     subject := relabeling_term mu23 (subject (relabeling_triple mu12 t));
+     predicate := predicate (relabeling_triple mu12 t);
+     object := relabeling_term mu23 (object (relabeling_triple mu12 t));
+     subject_in_IB := wfs2;
+     predicate_in_I := wfp3
+   |} = {|
+          subject := relabeling_term (mu23 \o mu12) (subject t);
+          predicate := predicate t;
+          object := relabeling_term (mu23 \o mu12) (object t);
+          subject_in_IB := wfs;
+          predicate_in_I := wfp
+        |}.
+                 move=> /(_ tin).
+                 move=> tin2.
+                 suffices ib : (is_in_ib (relabeling_term mu12 (subject t))).
+                 (* The term "ib" has type "is_true (is_in_ib (relabeling_term mu12 (subject t)))" while it is expected to have type "triple I B L". *)
+                 apply (mu12_part _ ib wfp2).
+                 suffices -> :  {|
+                              subject := relabeling_term mu12 (subject t);
+                                         predicate := predicate t;
+                                                      object := relabeling_term mu12 (object t);
+                                                                subject_in_IB := ib;
+                                                                                 predicate_in_I := wfp2
+                               |} = relabeling_triple mu12 t.
+                 by apply tin2.
+                 apply triple_inj=> /=.
+               + by rewrite projs_rel.
+               + by rewrite projp_rel; case : (predicate t) wfp2=> //.
+               + by rewrite projo_rel.
+             move: wfs {tin}.
+             by rewrite relabeling_term_comp -relabeling_term_preserves_is_in_ib.
+                 apply triple_inj=> /=.
+               + by rewrite projs_rel relabeling_term_comp.
+               + by rewrite projp_rel; case : (predicate t) wfp2=> //.
+               + by rewrite projo_rel relabeling_term_comp.
+               + rewrite -relabeling_seq_triple_comp /relabeling_seq_triple.
+                 have /eq_uniq -> //: size [seq relabeling_triple mu23 i | i <- [seq relabeling_triple mu12 i | i <- ts1]] =
+                               size (relabeling_seq_triple mu23 ts2).
+                 by move: perm12=> /perm_size; rewrite !size_map.
+                 by apply eq_mem_map; apply perm_mem.
       Qed.
 
       Lemma iso_trans g1 g2 g3 : iso g1 g2 -> iso g2 g3 -> iso g1 g3.
       Proof. by apply iso_ts_trans. Qed.
 
-      Lemma ts_pre_iso_iso ts mu (urel: uniq (relabeling_seq_triple mu ts)) :
-        is_pre_iso_ts ts (relabeling_seq_triple mu ts) mu ->
-          is_iso_ts ts (relabeling_seq_triple mu ts) mu.
-      Proof. by move=> pre_iso; rewrite /is_iso/is_iso_ts pre_iso urel /=; apply perm_refl. Qed.
+      (* TODO *)
+      (* Lemma ts_pre_iso_iso ts mu (urel: uniq (relabeling_seq_triple mu ts)) : *)
+      (*   is_pre_iso_ts ts (relabeling_seq_triple mu ts) mu -> *)
+      (*     is_iso_ts ts (relabeling_seq_triple mu ts) mu. *)
+      (* Proof. by move=> pre_iso; rewrite /is_iso/is_iso_ts pre_iso urel /=; apply perm_refl. Qed. *)
 
       Section Isocanonical.
 
@@ -1301,14 +1601,261 @@ Section OrderRdf.
   Proof. by move=> x y z; apply le_st_trans. Qed.
 
   Lemma rdf_leP ts1 ts2 : reflect (sort le_triple ts1 = sort le_triple ts2) (perm_eq ts1 ts2).
-  Proof.
-  apply perm_sortP.
-  + by apply le_triple_total.
-  + by apply le_triple_trans.
-  + by apply le_triple_anti.
-  Qed.
+  Proof. exact: Order.TotalTheory.perm_sort_leP ts1 ts2. Qed.
+
+  Lemma rdf_leP' ts1 ts2 : (sort le_triple ts1 = sort le_triple ts2) <-> (perm_eq ts1 ts2).
+  Proof. exact: Bool.reflect_iff (Order.TotalTheory.perm_sort_leP ts1 ts2). Qed.
 
 End OrderRdf.
+
+Section RDF_Spec.
+
+  Variable I B L : eqType.
+
+  Definition node_triple (t : triple I B L) : seq (term I B L) :=
+    [:: (subject t); (object t)].
+
+  Fixpoint fix_node_terms (ts : seq (triple I B L)) : seq (term I B L) :=
+    match ts with
+    | [::] => [::]
+    | t :: ts' => (node_triple t) ++ (fix_node_terms ts')
+    end.
+
+  Definition node_terms (ts : seq (triple I B L)) : seq (term I B L) :=
+    undup (fix_node_terms ts).
+
+  Lemma uniq_node_terms (ts : seq (triple I B L)) : uniq (node_terms ts).
+  Proof. by apply undup_uniq. Qed.
+
+  Definition bij_nodes (ts1 ts2 : seq (triple I B L)) mu : bool :=
+    bnode_map_bij (node_terms ts1) (node_terms ts2) mu.
+
+  Definition bnodes_to_bnodes (mu : term I B L -> term I B L) :=
+    forall (trm : term I B L), is_bnode trm -> is_bnode (mu trm).
+
+  Definition lit_to_lit (ts: seq (triple I B L)) (mu : term I B L -> term I B L) :=
+    forall (trm : term I B L), trm \in (node_terms ts) -> is_lit trm -> is_lit (mu trm).
+
+  Definition iri_to_iri (ts: seq (triple I B L)) (mu : term I B L -> term I B L) :=
+    forall (trm : term I B L), trm \in (node_terms ts) -> is_iri trm -> is_iri (mu trm).
+
+  Lemma rel_pres_ib (ts : seq (triple I B L)) (mu : term I B L -> term I B L) (trm : term I B L) :
+    bnodes_to_bnodes mu ->
+    iri_to_iri ts mu ->
+    trm \in (node_terms ts) ->
+            is_in_ib  trm ->
+            is_in_ib (mu trm).
+  Proof.
+  case: trm=> [i|l|b] btb iti in_node // iib; rewrite /is_in_ib.
+  + have := iti (Iri i) in_node. by move ->.
+  + have := btb (Bnode b). by rewrite Bool.orb_comm=> ->.
+  Qed.
+
+  Lemma rel_pres_i ts (mu : term I B L -> term I B L) (trm : term I B L) :
+    iri_to_iri ts mu -> trm \in (node_terms ts) ->
+                                is_in_i  trm -> is_in_i (mu trm).
+  Proof. by case: trm=> [i|l|b] iti in_node //=> /(iti (Iri i) in_node). Qed.
+
+  Definition spec_rel_triple_iso (t : triple I B L) (mu : term I B L -> term I B L)
+    (pres_s: is_in_ib (mu (subject t)))
+    (pres_p : is_in_i (predicate t)) : triple I B L :=
+    mkTriple (mu (object t)) pres_s pres_p.
+
+  Definition pres_wf (ts : seq (triple I B L)) (mu : term I B L -> term I B L) :=
+    forall trm,
+      trm \in (node_terms ts) ->
+        ( (is_in_ib trm -> is_in_ib (mu trm)) /\ (is_in_i trm -> is_in_i (mu trm))).
+
+  Definition rel_wf_triple (t : triple I B L) (mu : term I B L -> term I B L) (ts : seq (triple I B L))
+    (mu_pres_wf : pres_wf ts mu) : (subject t) \in (node_terms ts) -> triple I B L :=
+    (match t with
+       mkTriple s p o sib pii =>
+         fun sin => @mkTriple I B L (mu s) p (mu o) ((mu_pres_wf s sin).1 sib) pii
+     end).
+
+  Lemma in_nodes_cons (trm : term I B L) (ts : seq (triple I B L)) (t' : triple I B L):
+    trm \in node_terms ts -> trm \in node_terms (t' :: ts).
+  Proof.
+    by rewrite /node_terms !mem_undup=> H; rewrite /= !in_cons H !orbT. 
+  Qed.
+
+  Lemma in_triple_s_in_node_terms (t: triple I B L) (ts : seq (triple I B L)) :
+    t \in ts -> (subject t) \in (node_terms ts).
+  Proof.
+    elim: ts=> [|t' ts' IH]; first by rewrite in_nil.
+    rewrite in_cons. move=> /orP[/eqP->|].
+    by rewrite /node_terms undup_in // /fix_node_terms in_cons eqxx.
+    by move=> /IH; apply in_nodes_cons.
+  Qed.
+
+  Definition adj_pres (ts1 ts2: seq (triple I B L)) (mu : term I B L -> term I B L) :=
+    pres_wf ts1 mu ->
+    forall t, t \in ts1 <-> forall wf_s wf_p, @mkTriple I B L (mu (subject t)) (predicate t) (mu (object t)) wf_s wf_p \in ts2.
+
+  Definition spec_is_iso (ts1 ts2 : seq (triple I B L)) mu :=
+    bij_nodes ts1 ts2 mu /\
+      bnodes_to_bnodes mu /\
+        lit_to_lit ts1 mu /\
+          iri_to_iri ts1 mu /\
+            adj_pres ts1 ts2 mu.
+
+  Definition spec_iso (ts1 ts2 : seq (triple I B L)) :=
+    exists mu, spec_is_iso ts1 ts2 mu.
+
+  Lemma nodes_terms_cons (trpl : triple I B L) (ts : seq (triple I B L)):
+    node_terms (trpl :: ts) = undup (node_triple trpl ++ node_terms ts).
+  Proof. by rewrite {1}/node_terms /fix_node_terms -undup_cat_r -undup_cat_l. Qed.
+
+  Lemma bnodes_nodes (ts : seq (triple I B L)) : perm_eq (bnodes_ts ts) (filter (@is_bnode I B L) (node_terms ts)).
+  Proof.
+  suffices mem_eq : (bnodes_ts ts) =i (filter (@is_bnode I B L) (node_terms ts)).
+    apply uniq_perm=> //.
+    + by apply uniq_bnodes_ts.
+    + by apply filter_uniq; apply uniq_node_terms.
+  elim: ts=> [//| t tl IHl].
+  move=> T; rewrite bnodes_ts_cons mem_undup.
+  rewrite nodes_terms_cons filter_undup mem_undup filter_cat.
+  rewrite !mem_cat.
+  f_equal ; last by rewrite IHl.
+  case: t=> s p o sib pii. rewrite /bnodes_triple.
+  rewrite /terms_triple filter_undup mem_undup.
+  suffices -> : [seq x <- [:: s; p; o] | is_bnode x] = [seq x <- [:: s; o] | is_bnode x].
+    done.
+  by case: p pii=> //.
+  Qed.
+
+  Lemma map_filter_nodes ts (mu : B -> B)  :
+    [seq x <- [seq relabeling_term mu i | i <- node_terms ts] | is_bnode x] = [seq relabeling_term mu i | i <- [seq x <- node_terms ts | is_bnode x]].
+  Proof. by elim: (node_terms ts) => [//| []h tl IHl]; rewrite /= IHl. Qed.
+
+  (* Lemma relabeling_nodes ts (mu : B -> B)  : *)
+  (*   [seq relabeling_term mu i | i <- node_terms ts] = *)
+  (*     node_terms (relabeling_seq_triple mu ts). *)
+  (* Proof. elim: ts=> [//| h tl IHl]. rewrite /=. rewrite !nodes_terms_cons. *)
+
+  Theorem iso_equiv (ts1 ts2 : seq (triple I B L)) :
+    (uniq ts1) -> (uniq ts2) ->
+      iso_ts ts1 ts2 <-> spec_iso ts1 ts2.
+  Proof.
+  move=> u1 u2; split.
+  move=> [mu [/and3P[piso wf_ret adj]] mu_part].
+  exists (relabeling_term mu); split.
+  have piso2 := piso.
+  rewrite /is_pre_iso_ts/bnode_map_bij in piso.
+  move : piso => /and3P[_ _ piso].
+  (* apply (perm_map (@Bnode I B L)) in piso. *)
+  rewrite /bij_nodes.
+  rewrite /bnode_map_bij.
+  rewrite !uniq_node_terms /=.
+  have bnG := bnodes_nodes ts1.
+  have bnH := bnodes_nodes ts2.
+  have /permEl nodes_filterG := perm_filterC (@is_bnode I B L) (node_terms ts2).
+  suffices H : perm_eq (map (relabeling_term mu) (node_terms ts1)) ([seq x <- node_terms ts2 | is_bnode x] ++ [seq x <- node_terms ts2 | predC (is_bnode (L:=L)) x]) .
+    by apply (perm_trans H nodes_filterG).
+    have /permEl nodes_filterH := perm_filterC (@is_bnode I B L) (map (relabeling_term mu) (node_terms ts1)).
+    eapply perm_trans. rewrite perm_sym. apply nodes_filterH.
+    apply perm_cat.
+    suffices H : perm_eq [seq x <- [seq relabeling_term mu i | i <- node_terms ts1] | is_bnode x] (bnodes_ts ts2).
+    eapply perm_trans. apply H. apply bnH.
+
+    rewrite perm_sym.
+    eapply perm_trans.
+    rewrite -perm_relabel_bts perm_sym in piso.
+    apply piso.
+    rewrite filter_map.
+    apply perm_map.
+    elim: ts1 {u1 wf_ret adj mu_part piso2 piso bnG nodes_filterH}=> [//|[]s p o sib pii tl IHl] //=.
+    rewrite bnodes_ts_cons. rewrite nodes_terms_cons. rewrite filter_undup.
+    apply perm_undup.
+    move=> t. rewrite filter_cat. rewrite !mem_cat. rewrite (perm_mem IHl). f_equal.
+    rewrite /bnodes_triple/terms_triple.
+    rewrite filter_undup mem_undup.
+    rewrite /node_triple. 
+    case: s sib=> //=; case : p pii=> //=; case: o=> //=.
+    move=> {bnG bnH nodes_filterG nodes_filterH}.
+    suffices H : uniq  [seq x <- [seq relabeling_term mu i | i <- node_terms ts1] | predC (is_bnode (L:=L)) x].
+    suffices H2 : uniq [seq x <- node_terms ts2 | predC (is_bnode (L:=L)) x].
+      rewrite -(undup_id H) -(undup_id H2).
+      apply perm_undup=> t.
+
+    apply (perm_mem IHl).
+
+    rewrite filter_map.
+    admit.
+    apply (perm_map (relabeling_term mu)) in bnG.
+
+    apply bnH.
+    suffices H : perm_eq [seq x <- [seq relabeling_term mu i | i <- node_terms ts1] | is_bnode x] (bnodes_ts ts2).
+
+    rewrite map_filter_nodes.
+    rewrite filter_map.
+    apply perm_map
+
+   admit.
+   apply nodes_filterG.
+  (* rewrite -perm_relabel_bts in piso. *)
+  apply uniq_perm.
+  have equ := perm_uniq piso.
+  rewrite map_inj_in_uniq.
+  by rewrite -(perm_uniq bnG) uniq_bnodes_ts.
+  have piso_inj := (is_pre_iso_ts_inj piso2).
+  move=> /= x y.
+  rewrite -!(perm_mem bnG).
+  case: x=> // bx.
+  - by rewrite i_in_bnodes_ts.
+  - by rewrite l_in_bnodes_ts.
+  case: y => // by1.
+  rewrite !bnodes_map_get_bts.
+  rewrite !mem_map.
+  move=> bxin byin.
+  rewrite /==> [[]].
+  move=> /piso_inj=> -> //.
+  by move=> x y []. 
+  by move=> x y [].
+  by rewrite -(perm_uniq bnH) uniq_bnodes_ts.
+  move=> b.
+  rewrite -(perm_mem bnH).
+  rewrite -(eq_mem_map (relabeling_term mu) (perm_mem bnG)).
+  rewrite -perm_relabel_bts in piso.
+  apply (perm_mem piso).
+  (*  *)
+  + split.
+  + by move=> []//.
+  + split.
+    - by move=> []//.
+    - split.
+      * by move=> []//.
+        ++ rewrite /adj_pres/pres_wf /==> p_wf t; split=> tin.
+          move=> wf_s wf_p.
+          apply perm_mem in adj.
+          rewrite -adj.
+          suffices -> : {|
+                       subject := relabeling_term mu (subject t);
+                                  predicate := predicate t;
+                                               object := relabeling_term mu (object t);
+                                                         subject_in_IB := wf_s;
+                                                                          predicate_in_I := wf_p
+                     |} = relabeling_triple mu t.
+            by apply map_f.
+          apply triple_inj; case: t tin wf_s wf_p=> /= s p o sib pin tin wf_s wf_p //.
+          by case: p pin tin wf_p.
+        suffices [wfs wfp]: is_in_ib (relabeling_term mu (subject t)) /\ is_in_i (predicate t).
+          by apply (mu_part _ wfs wfp); apply tin.
+        split.
+         + case t=> s /= _ _ sib _. by apply relabeling_term_preserves_is_in_ib.
+         + by case t=> _ p /= _ _ pii.
++ move=> [mu_trm [b_to_b [l_id [i_id /= adj_pres]]]].
+  rewrite /adj_pres/= in adj_pres.
+  rewrite /iso_ts/is_iso_ts.
+  have : exists nu, 
+
+   spec_is_iso ts1 ts2 mu_trm
+
+
+
+
+
+End RDF_Spec.
 
 End Rdf.
 
